act1/theories/Types.v
@@ -10,6 +10,96 @@ Require Import MiniEMTST.AtomScopes.
 Require Import MiniEMTST.Syntax.
 Require Import MiniEMTST.Env.
 
+(* syntax of types *)
+
+(** types **)
+
+Inductive sort : Set :=
+  | boole : sort. (* boolean expression *)
+
+Fixpoint eq_sort (s s' : sort) : bool :=
+  match s, s' with
+  | boole, boole => true
+  (* | _, _ => false *) (* there is only one type for now *)
+  end.
+
+Lemma eq_sortP : Equality.axiom eq_sort.
+Proof.
+  move=> x y.
+  apply: (iffP idP)=>[|<-].
+  by elim x ; elim y.
+  by elim x.
+Qed.
+
+Canonical sort_eqMixin := EqMixin eq_sortP.
+Canonical sort_eqType := Eval hnf in EqType sort sort_eqMixin.
+
+Inductive tp : Set :=
+  | input : sort -> tp -> tp
+  | output : sort -> tp -> tp
+  | ended : tp
+  | bottom : tp
+.
+
+Fixpoint dual (T : tp) : tp :=
+  match T with
+  | input s T => output s (dual T)
+  | output s T => input s (dual T)
+  | ended => ended
+  | bottom => bottom
+  end
+.
+
+Lemma dual_is_dual t : dual (dual t) = t.
+  elim t=>// ; rewrite/dual ; move=>//; rewrite-/dual ;
+    do ? (move=> s t0 =>->) ;
+    do ? (move=> t0 R' t1 =>->) ;
+    rewrite ?R' ;
+   easy.
+Qed.
+
+Fixpoint eq_tp (T T': tp) : bool :=
+  match T, T' with
+  | input s T, input s' T' => eq_sort s s' && eq_tp T T'
+  | output s T, output s' T' => eq_sort s s' && eq_tp T T'
+  | ended, ended => true
+  | bottom, bottom => true
+  | _, _ => false
+  end.
+
+Lemma eq_imp_eq : forall x y, eq_tp x y -> x = y.
+Proof. Admitted.
+(*   apply tp_sort_mutind ; intros; try destruct y  ; try destruct s'; try easy ; *)
+(*   inversion H1 ; apply Bool.andb_true_iff in H3 ; destruct H3 ; *)
+(*   try(move:H3 ; move/H0=>H3 ; move:H2 ; move/H=>H4 ; by rewrite H3 H4). *)
+(* Qed. (* more ssreflect can make this better *) *)
+
+Lemma eq_tp_refl x : eq_tp x x.
+Proof.
+  elim x ;
+    try
+      move=>s t H ;
+      rewrite/eq_tp=>// ;
+      fold eq_tp ;
+      rewrite H=>//= ;
+      elim s=>//.
+Qed.
+
+
+Lemma eq_tpP : Equality.axiom eq_tp.
+Proof.
+  move=>x y.
+  apply: (iffP idP)=>[|<-].
+  apply eq_imp_eq.
+  apply eq_tp_refl.
+Qed.
+
+
+Canonical tp_eqMixin := EqMixin eq_tpP.
+Canonical tp_eqType := Eval hnf in EqType tp tp_eqMixin.
+
+(* judgements *)
+
 Definition sort_env_entry := EV_atom_ordType.
 Definition sort_env := @env sort_env_entry sort_eqType.
 
